pcuic/theories/PCUICLiftSubst.v
@@ -2,7 +2,7 @@
 
 From Coq Require Import List Program.
 From Template Require Import utils Ast.
-From PCUIC Require Import Ast AstUtils Induction.
+From PCUIC Require Import PCUICAst PCUICAstUtils PCUICInduction.
 From Coq Require Import BinPos Arith.Compare_dec Bool Lia.
 
 (** * Lifting and substitution for the AST
@@ -238,8 +238,8 @@ Ltac nth_leb_simpl :=
   | |- context [nth_error ?l ?n] => elim (nth_error_spec l n); rewrite -> ?app_length, ?map_length;
                                     try lia; intros; simpl
   | H : context[nth_error (?l ++ ?l') ?n] |- _ =>
-    (rewrite -> (AstUtils.nth_error_app_ge l l' n) in H by lia) ||
-    (rewrite -> (AstUtils.nth_error_app_lt l l' n) in H by lia)
+    (rewrite -> (PCUICAstUtils.nth_error_app_ge l l' n) in H by lia) ||
+    (rewrite -> (PCUICAstUtils.nth_error_app_lt l l' n) in H by lia)
   | H : nth_error ?l ?n = Some _, H' : nth_error ?l ?n' = Some _ |- _ =>
     replace n' with n in H' by lia; rewrite -> H in H'; injection H'; intros; subst
   | _ => lia || congruence || solve [repeat (f_equal; try lia)]
