pcuic/theories/PCUICRetyping.v
@@ -2,7 +2,7 @@
 
 From Coq Require Import Bool String List Program BinPos Compare_dec Omega.
 From Template Require Import config monad_utils utils Ast univ.
-From PCUIC Require Import Ast AstUtils Induction LiftSubst UnivSubst Typing Checker.
+From PCUIC Require Import PCUICAst PCUICAstUtils PCUICInduction PCUICLiftSubst PCUICUnivSubst PCUICTyping PCUICChecker.
 Require Import String.
 Local Open Scope string_scope.
 Set Asymmetric Patterns.
