pcuic/theories/PCUICWcbvEval.v
@@ -2,9 +2,7 @@
 
 From Coq Require Import Bool String List Program BinPos Compare_dec Omega.
 From Template Require Import config utils univ Ast.
-From PCUIC Require Import Ast AstUtils Induction.
-From PCUIC Require Import LiftSubst UnivSubst.
-From PCUIC Require Import Typing.
+From PCUIC Require Import PCUICAst PCUICAstUtils PCUICInduction PCUICLiftSubst PCUICUnivSubst PCUICTyping.
 Require Import String.
 Local Open Scope string_scope.
 Set Asymmetric Patterns.
